pcuic/theories/Bidirectional/BDStrengthening.v
@@ -2,6 +2,7 @@ From Coq Require Import Bool List Arith Lia.
 From Coq Require String.
 From MetaCoq.Template Require Import config utils monad_utils.
 From MetaCoq.PCUIC Require Import PCUICAst PCUICAstUtils PCUICGlobalEnv 
+  PCUICTactics
   PCUICInduction PCUICLiftSubst PCUICUnivSubst PCUICEquality PCUICUtils
   PCUICPosition PCUICTyping PCUICSigmaCalculus PCUICOnFreeVars PCUICClosed PCUICConfluence PCUICSpine PCUICInductiveInversion PCUICParallelReductionConfluence PCUICWellScopedCumulativity PCUICClosed PCUICRenameDef PCUICInstConv PCUICClosedTyp PCUICWeakeningEnvTyp PCUICRenameTyp PCUICRenameConv PCUICGuardCondition PCUICWeakeningConv.
 
